Rename _special -> _borrow

theories/region_invariants.v
@@ -200,9 +200,9 @@ Section heap.
         ⌜ related_sts_priv_world W W'⌝
         → φ (W,C,v) -∗ φ (W',C,v))%I.
 
-  Definition future_special_mono (C : CmptName) (φ : (WORLD * CmptName * Word) -> iProp Σ) (v  : Word) : iProp Σ :=
+  Definition future_borrow_mono (C : CmptName) (φ : (WORLD * CmptName * Word) -> iProp Σ) (v  : Word) : iProp Σ :=
     (□ ∀ (W W' : WORLD),
-        ⌜ related_sts_special_world W W'⌝
+        ⌜ related_sts_borrow_world W W'⌝
         → φ (W,C,v) -∗ φ (W',C,v))%I.
 
   Lemma future_priv_mono_is_future_pub_mono (C : CmptName) (φ: (WORLD * CmptName * Word) → iProp Σ) v :
@@ -214,28 +214,28 @@ Section heap.
     iPureIntro; eauto using related_sts_pub_priv_world.
   Qed.
 
-  Lemma future_priv_mono_is_future_special_mono (C : CmptName) (φ: (WORLD * CmptName * Word) → iProp Σ) v :
-    future_priv_mono C φ v -∗ future_special_mono C φ v.
+  Lemma future_priv_mono_is_future_borrow_mono (C : CmptName) (φ: (WORLD * CmptName * Word) → iProp Σ) v :
+    future_priv_mono C φ v -∗ future_borrow_mono C φ v.
   Proof.
-    iIntros "#H". unfold future_special_mono. iModIntro.
+    iIntros "#H". unfold future_borrow_mono. iModIntro.
     iIntros (W W' Hrelated) "Hφ".
     iApply "H"; eauto.
-    iPureIntro; eauto using related_sts_special_priv_world.
+    iPureIntro; eauto using related_sts_borrow_priv_world.
   Qed.
 
-  Lemma future_special_mono_is_future_pub_mono (C : CmptName) (φ: (WORLD * CmptName * Word) → iProp Σ) v :
-    future_special_mono C φ v -∗ future_pub_mono C φ v.
+  Lemma future_borrow_mono_is_future_pub_mono (C : CmptName) (φ: (WORLD * CmptName * Word) → iProp Σ) v :
+    future_borrow_mono C φ v -∗ future_pub_mono C φ v.
   Proof.
     iIntros "#H". unfold future_pub_mono. iModIntro.
     iIntros (W W' Hrelated) "Hφ".
     iApply "H"; eauto.
-    iPureIntro; eauto using related_sts_pub_special_world.
+    iPureIntro; eauto using related_sts_pub_borrow_world.
   Qed.
 
   Definition mono_pub (C : CmptName) (φ : (WORLD * CmptName * Word) -> iProp Σ) :=
     (∀ (w : Word), future_pub_mono C φ w)%I.
-  Definition mono_special (C : CmptName) (φ : (WORLD * CmptName * Word) -> iProp Σ) (p : Perm) :=
-    (∀ (w : Word), ⌜canStore p w = true⌝ -∗ future_special_mono C φ w)%I.
+  Definition mono_borrow (C : CmptName) (φ : (WORLD * CmptName * Word) -> iProp Σ) (p : Perm) :=
+    (∀ (w : Word), ⌜canStore p w = true⌝ -∗ future_borrow_mono C φ w)%I.
   Definition mono_priv (C : CmptName) (φ : (WORLD * CmptName * Word) -> iProp Σ) (p : Perm) :=
     (∀ (w : Word), ⌜canStore p w = true⌝ -∗ future_priv_mono C φ w)%I.
 
@@ -295,11 +295,11 @@ Section heap.
     iApply (future_priv_mono_eq_pred with "Hφ Hφ' Hmono");auto.
   Qed.
 
-  Lemma future_special_mono_eq_pred C γ φ φ' w :
+  Lemma future_borrow_mono_eq_pred C γ φ φ' w :
     saved_pred_own γ DfracDiscarded φ
     -∗ saved_pred_own γ DfracDiscarded φ'
-    -∗ ▷ future_special_mono C φ w
-    -∗ ▷ future_special_mono C φ' w.
+    -∗ ▷ future_borrow_mono C φ w
+    -∗ ▷ future_borrow_mono C φ' w.
   Proof.
     iIntros "#Hφ #Hφ' #Hmono".
     iIntros (W0 W1 Hrelated).
@@ -311,16 +311,16 @@ Section heap.
     iApply "Hmono"; eauto.
   Qed.
 
-  Lemma mono_special_eq_pred C γ p φ φ':
+  Lemma mono_borrow_eq_pred C γ p φ φ':
     saved_pred_own γ DfracDiscarded φ
     -∗ saved_pred_own γ DfracDiscarded φ'
-    -∗ ▷ mono_special C φ p
-    -∗ ▷ mono_special C φ' p.
+    -∗ ▷ mono_borrow C φ p
+    -∗ ▷ mono_borrow C φ' p.
   Proof.
     iIntros "#Hφ #Hφ' #Hmono".
     iIntros (w Hglobalw).
     iSpecialize ("Hmono" $! w Hglobalw).
-    iApply (future_special_mono_eq_pred with "Hφ Hφ' Hmono");auto.
+    iApply (future_borrow_mono_eq_pred with "Hφ Hφ' Hmono");auto.
   Qed.
 
   (* Asserting that a location is in a specific state in a given World *)
@@ -368,7 +368,7 @@ Section heap.
                                         ∗ (if isWL p
                                            then future_pub_mono C φ v
                                            else (if isDL p
-                                                 then future_special_mono C φ v
+                                                 then future_borrow_mono C φ v
                                                  else future_priv_mono C φ v)
                                           )
                                         ∗ ▷ φ (W,C,v)
@@ -376,7 +376,7 @@ Section heap.
                           ∃ (v : Word), ⌜isO p = false⌝
                                         ∗ a ↦ₐ v
                                         ∗ (if isDL p
-                                                 then future_special_mono C φ v
+                                                 then future_borrow_mono C φ v
                                                  else future_priv_mono C φ v)
                                         ∗ ▷ φ (W,C,v)
                       | Frozen m =>
@@ -588,11 +588,11 @@ Section heap.
     iApply (future_priv_mono_eq_pred_rel with "Hrel Hrel' Hmono"); eauto.
   Qed.
 
-  Lemma future_special_mono_eq_pred_rel C γ p p' φ φ' w :
+  Lemma future_borrow_mono_eq_pred_rel C γ p p' φ φ' w :
     rel C γ p φ
     -∗ rel C γ p' φ'
-    -∗ ▷ future_special_mono C φ w
-    -∗ ▷ future_special_mono C φ' w.
+    -∗ ▷ future_borrow_mono C φ w
+    -∗ ▷ future_borrow_mono C φ' w.
   Proof.
     iIntros "#Hrel #Hrel' #Hmono".
     iIntros (W0 W1 Hrelated).
@@ -605,16 +605,16 @@ Section heap.
     iApply "Hmono"; eauto.
   Qed.
 
-  Lemma mono_special_eq_pred_rel C γ p p' φ φ' :
+  Lemma mono_borrow_eq_pred_rel C γ p p' φ φ' :
     rel C γ p φ
     -∗ rel C γ p' φ'
-    -∗ ▷ mono_special C φ p
-    -∗ ▷ mono_special C φ' p.
+    -∗ ▷ mono_borrow C φ p
+    -∗ ▷ mono_borrow C φ' p.
   Proof.
     iIntros "#Hrel #Hrel' #Hmono".
     iIntros (w Hglobalw).
     iSpecialize ("Hmono" $! w Hglobalw).
-    iApply (future_special_mono_eq_pred_rel with "Hrel Hrel' Hmono"); eauto.
+    iApply (future_borrow_mono_eq_pred_rel with "Hrel Hrel' Hmono"); eauto.
   Qed.
 
 
@@ -636,14 +636,14 @@ Section heap.
       iDestruct "Hl" as (v Hne) "(Hl & #HmonoV & Hφ)".
       iFrame "%#∗".
       destruct (isWL p); [| destruct (isDL p)]; (iApply "HmonoV"; eauto; iFrame).
-      + iPureIntro; apply related_sts_pub_special_world in Hrelated; naive_solver.
+      + iPureIntro; apply related_sts_pub_borrow_world in Hrelated; naive_solver.
       + iPureIntro; apply related_sts_pub_priv_world in Hrelated; naive_solver.
     - iDestruct "Hm" as (γpred p φ Heq Hpers) "(#Hsavedφ & Hl)".
       iDestruct "Hl" as (v Hne) "(Hl & #HmonoV & Hφ)".
       iFrame "%#∗".
       destruct (isDL p);
       iApply "HmonoV"; iFrame "∗#"; auto.
-      + iPureIntro; apply related_sts_pub_special_world in Hrelated; naive_solver.
+      + iPureIntro; apply related_sts_pub_borrow_world in Hrelated; naive_solver.
       + iPureIntro; apply related_sts_pub_priv_world in Hrelated; naive_solver.
     - done.
     - done.
@@ -825,7 +825,7 @@ Section heap.
            ∗ sts_state_std C l Temporary
            ∗ l ↦ₐ v
            ∗ ⌜isO p = false⌝
-           ∗ ▷ (if isDL p then future_special_mono C φ v else future_priv_mono C φ v)
+           ∗ ▷ (if isDL p then future_borrow_mono C φ v else future_priv_mono C φ v)
            ∗ ▷ φ (W,C,v).
   Proof.
     iIntros (Htemp Hpwl) "(#Hrel & Hreg & Hfull)".
@@ -853,7 +853,7 @@ Section heap.
     - repeat (iSplitR).
       + auto.
       + destruct (isDL p').
-        * iApply future_special_mono_eq_pred; auto.
+        * iApply future_borrow_mono_eq_pred; auto.
         * iApply future_priv_mono_eq_pred; auto.
       + iNext; iRewrite "Hφeq". iFrame "∗ #".
   Qed.
@@ -910,7 +910,7 @@ Section heap.
            ∗ sts_state_std C l Permanent
            ∗ l ↦ₐ v
            ∗ ⌜isO p = false⌝
-           ∗ ▷ (if isDL p then future_special_mono C φ v else future_priv_mono C φ v)
+           ∗ ▷ (if isDL p then future_borrow_mono C φ v else future_priv_mono C φ v)
            ∗ ▷ φ (W,C,v).
   Proof.
     iIntros (Htemp) "(#Hrel & Hreg & Hfull)".
@@ -938,7 +938,7 @@ Section heap.
     - repeat (iSplitR).
       + auto.
       + destruct (isDL p').
-        * iApply future_special_mono_eq_pred; auto.
+        * iApply future_borrow_mono_eq_pred; auto.
         * iApply future_priv_mono_eq_pred; auto.
       + iNext; iRewrite "Hφeq". iFrame "∗ #".
   Qed.
@@ -983,8 +983,8 @@ Section heap.
          ∗ (▷ if (decide (ρ = Temporary))
               then ( if isWL p
                      then future_pub_mono C φ v
-                     else (if isDL p then future_special_mono C φ v else future_priv_mono C φ v))
-              else (if isDL p then future_special_mono C φ v else future_priv_mono C φ v))
+                     else (if isDL p then future_borrow_mono C φ v else future_priv_mono C φ v))
+              else (if isDL p then future_borrow_mono C φ v else future_priv_mono C φ v))
          ∗ ▷ φ (W,C,v).
   Proof.
     iIntros (Hne Htemp) "(Hrel & Hreg & Hfull)".
@@ -1168,7 +1168,7 @@ Section heap.
     ∗ open_region W C a
     ∗ a ↦ₐ v
     ∗ ⌜isO p = false⌝
-    ∗ (if isDL p then future_special_mono C φ v else future_priv_mono C φ v)
+    ∗ (if isDL p then future_borrow_mono C φ v else future_priv_mono C φ v)
     ∗ ▷ φ (W,C,v)
     ∗ rel C a p φ
     -∗ region W C.
@@ -1254,7 +1254,7 @@ Section heap.
       ∗ open_region W C a
       ∗ a ↦ₐ v
       ∗ ⌜isO p = false⌝
-      ∗ (if isDL p then future_special_mono C φ v else future_priv_mono C φ v)
+      ∗ (if isDL p then future_borrow_mono C φ v else future_priv_mono C φ v)
       ∗ ▷ φ (W,C,v)
       ∗ rel C a p φ
       -∗ region W C.
@@ -1285,8 +1285,8 @@ Section heap.
     ∗ (if (decide (ρ = Temporary))
        then ( if isWL p
               then future_pub_mono C φ v
-              else (if isDL p then future_special_mono C φ v else future_priv_mono C φ v))
-       else (if isDL p then future_special_mono C φ v else future_priv_mono C φ v))
+              else (if isDL p then future_borrow_mono C φ v else future_priv_mono C φ v))
+       else (if isDL p then future_borrow_mono C φ v else future_priv_mono C φ v))
     ∗ ▷ φ (W,C,v)
     ∗ rel C a p φ
       -∗ region W C.
@@ -1402,7 +1402,7 @@ Section heap.
          ∗ sts_state_std C a Temporary
          ∗ a ↦ₐ v
          ∗ ⌜isO p = false⌝
-         ∗ ▷ (if isDL p then future_special_mono C φ v else future_priv_mono C φ v)
+         ∗ ▷ (if isDL p then future_borrow_mono C φ v else future_priv_mono C φ v)
          ∗ ▷ φ (W,C,v).
   Proof.
     rewrite open_region_many_eq .
@@ -1431,7 +1431,7 @@ Section heap.
     - repeat (iSplitR).
       + auto.
       + destruct (isDL p').
-        * iApply future_special_mono_eq_pred; auto.
+        * iApply future_borrow_mono_eq_pred; auto.
         * iApply future_priv_mono_eq_pred; auto.
       + iNext; iRewrite "Hφeq". iFrame.
   Qed.
@@ -1447,7 +1447,7 @@ Section heap.
         ∗ open_region_many W C (a :: als)
         ∗ a ↦ₐ v
         ∗ ⌜isO p = false⌝
-        ∗ ▷ (if isDL p then future_special_mono C φ v else future_priv_mono C φ v)
+        ∗ ▷ (if isDL p then future_borrow_mono C φ v else future_priv_mono C φ v)
         ∗ ▷ φ (W,C,v).
   Proof.
     rewrite open_region_many_eq .
@@ -1477,7 +1477,7 @@ Section heap.
     - repeat (iSplitR).
       + auto.
       + destruct (isDL p').
-        * iApply future_special_mono_eq_pred; auto.
+        * iApply future_borrow_mono_eq_pred; auto.
         * iApply future_priv_mono_eq_pred; auto.
       + iNext; iRewrite "Hφeq". iFrame.
   Qed.
@@ -1587,7 +1587,7 @@ Section heap.
     ∗ open_region_many W C (a::als)
     ∗ a ↦ₐ v
     ∗ ⌜isO p = false⌝
-    ∗ (if isDL p then future_special_mono C φ v else future_priv_mono C φ v)
+    ∗ (if isDL p then future_borrow_mono C φ v else future_priv_mono C φ v)
     ∗ ▷ φ (W,C,v)
     ∗ rel C a p φ
       -∗ open_region_many W C als.
@@ -1666,7 +1666,7 @@ Section heap.
     ∗ open_region_many W C (a::als)
     ∗ a ↦ₐ v
     ∗ ⌜isO p = false⌝
-    ∗ (if isDL p then future_special_mono C φ v else future_priv_mono C φ v)
+    ∗ (if isDL p then future_borrow_mono C φ v else future_priv_mono C φ v)
     ∗ ▷ φ (W,C,v)
     ∗ rel C a p φ
       -∗ open_region_many W C als.
@@ -1698,8 +1698,8 @@ Section heap.
     (C : CmptName) (φ : WORLD * CmptName * Word → iProp Σ)
     (p : Perm) (w : Word) (ρ : region_type) :=
     (match ρ with
-     | Temporary => (if isWL p then future_pub_mono else (if isDL p then future_special_mono else future_priv_mono))
-     | Permanent => (if isDL p then future_special_mono else future_priv_mono)
+     | Temporary => (if isWL p then future_pub_mono else (if isDL p then future_borrow_mono else future_priv_mono))
+     | Permanent => (if isDL p then future_borrow_mono else future_priv_mono)
      | Revoked | Frozen _ => λ _ _ _, True
      end C φ w)%I.
 
@@ -1707,8 +1707,8 @@ Section heap.
     (C : CmptName) (φ : WORLD * CmptName * Word → iProp Σ)
     (p : Perm) (w : Word) (ρ : region_type) :=
     (if decide (ρ = Temporary)
-     then (if isWL p then future_pub_mono C φ w else (if isDL p then future_special_mono C φ w else future_priv_mono C φ w))
-     else (if isDL p then future_special_mono C φ w else future_priv_mono C φ w) )%I.
+     then (if isWL p then future_pub_mono C φ w else (if isDL p then future_borrow_mono C φ w else future_priv_mono C φ w))
+     else (if isDL p then future_borrow_mono C φ w else future_priv_mono C φ w) )%I.
 
   (*Lemma that allows switching between the two different formulations of monotonicity, to alleviate the effects of inconsistencies*)
   Lemma switch_monotonicity_formulation
