theories/region_invariants_allocation.v
@@ -87,7 +87,7 @@ Section region_alloc.
     isO p = false ->
      a ∉ dom (std W) →
      (isWL p) = false →
-     (if isDL p then future_special_mono C φ v else future_priv_mono C φ v) -∗
+     (if isDL p then future_borrow_mono C φ v else future_priv_mono C φ v) -∗
      sts_full_world W C -∗
      region W C -∗
      a ↦ₐ v -∗
@@ -133,7 +133,7 @@ Section region_alloc.
         iFrame "∗ #".
         repeat(iSplitR;[auto|]).
         destruct (isDL p); iApply "HmonoV"; eauto.
-        + by iPureIntro; apply related_sts_pub_special_world.
+        + by iPureIntro; apply related_sts_pub_borrow_world.
         + by iPureIntro; apply related_sts_pub_priv_world.
       }
       iApply (big_sepM_mono with "Hpreds'").
@@ -153,7 +153,7 @@ Section region_alloc.
   Lemma extend_region_perm E W C a v p φ `{∀ Wv, Persistent (φ Wv)}:
     isO p = false ->
      a ∉ dom (std W) →
-     (if isDL p then future_special_mono C φ v else future_priv_mono C φ v) -∗
+     (if isDL p then future_borrow_mono C φ v else future_priv_mono C φ v) -∗
      sts_full_world W C -∗
      region W C -∗
      a ↦ₐ v -∗
@@ -198,7 +198,7 @@ Section region_alloc.
         iExists γpred,p,φ. iFrame "∗ #".
         repeat (iSplitR;[done|]).
         destruct (isDL p); iApply "HmonoV"; eauto.
-        + by iPureIntro; apply related_sts_pub_special_world.
+        + by iPureIntro; apply related_sts_pub_borrow_world.
         + by iPureIntro; apply related_sts_pub_priv_world.
       }
       iApply (big_sepM_mono with "Hpreds'").
@@ -328,7 +328,7 @@ Section region_alloc.
     -∗ ([∗ list] k;v ∈ l1;l2,
           k ↦ₐ v
           ∗ φ (W, C, v)
-          ∗ (if isDL p then future_special_mono C φ v else future_priv_mono C φ v))
+          ∗ (if isDL p then future_borrow_mono C φ v else future_priv_mono C φ v))
 
     ={E}=∗
 
@@ -365,7 +365,7 @@ Section region_alloc.
     ([∗ list] k;v ∈ l1;l2,
        k ↦ₐ v
        ∗ φ (W, C, v)
-       ∗ (if isDL p then future_special_mono C φ v else future_priv_mono C φ v)
+       ∗ (if isDL p then future_borrow_mono C φ v else future_priv_mono C φ v)
        ∗ rel C k p φ)
 
     ={E}=∗
